## Exercise 2.63

### Part A

```
(tree->list-1 tree1)
;Value: (1 3 5 7 9 11)
(tree->list-2 tree1)
;Value: (1 3 5 7 9 11)
(tree->list-1 tree2)
;Value: (1 3 5 7 9 11)
(tree->list-2 tree2)
;Value: (1 3 5 7 9 11)
(tree->list-1 tree3)
;Value: (1 3 5 7 9 11)
(tree->list-2 tree3)
;Value: (1 3 5 7 9 11)
```

Both procedures will return a list that begins with the leftmost leaf node of the tree, and ends with the rightmost.

So they produce the same ordered result for a given tree.

### Part B

Both operations must visit every node, which suggests order of growth O(n) or greater.

For tree->list-1, use of append is expensive. We must traverse the left sublist for every n nodes. The append operation will be O(log n) on average for a balanced tree, as the left sublist halves in size at each level. So we perform O(log n) of work at each of the n nodes, giving O(n log n) overall.

For tree->list-2, we cache the result with cons, which is cheaper, O(1). We iterate this way for every node which gives O(n).