## Exercise 1.19

### Part A - Proof

Apply transformation to $a$ and $b$

$$
b'=bp+aq
a'=bq+aq+ap
$$

Apply same transformation again to $b$

$$
b''=b'p+a'q
$$

$$
b''=(bp+aq)p+(bq+aq+ap)q
$$
$$
b''=bp^2+2aqp+bq^2+aq^2
$$
$$
b''=b(p^2+q^2)+a(2qp+q^2)
$$

Let $b''=bp' +aq'$

$$
bp' +aq'=b(p^2+q^2)+a(2qp+q^2)
$$

$$
p'=p^2+q^2, q'=2qp+q^2
$$

### Part B - Procedure

Here I have substituted in the expressions found for $p'$ and $q'$

```
(define (fib n)
  (fib-iter 1 0 0 1 n))

(define (fib-iter a b p q count)
  (cond ((= count 0) b)
        ((even? count)
         (fib-iter a
                   b
                   (+ (square p) (square q))
                   (+ (* 2 q p) (square q))
                   (/ count 2)))
        (else (fib-iter (+ (* b q) (* a q) (* a p))
                        (+ (* b p) (* a q))
                        p
                        q
                        (- count 1)))))
```
